Stumpling around more nontermination proofs

sandbox/nontermination.v
@@ -1,3 +1,5 @@
+Require Import Coq.Program.Equality.
+
 Inductive code : Set :=
   | AP : code -> code -> code
   | TOP : code
@@ -15,15 +17,21 @@ Inductive probe : code -> code -> Prop :=
 
 Inductive beta : code -> code -> Prop :=
   | beta_refl x : beta x x
-  (* this makes it difficult to prove the [head_beat_bot] lemma below
-  | beta_sym x y : beta y x -> beta x y
-  *)
   | beta_trans x y z : beta x y -> beta y z -> beta x z
   | beta_ap_left x x' y : beta x x' -> beta (x * y) (x' * y)
   | beta_ap_right x y y' : beta y y' -> beta (x * y) (x * y')
   | beta_i x : beta (I * x) x
   | beta_k x y : beta (K * x * y) x
   | beta_s x y z : beta (S * x * y * z) (x * z * (y * z)).
+Hint Constructors beta.
+
+Inductive beta_step : code -> code -> Prop :=
+  | beta_step_ap_left x x' y : beta_step x x' -> beta_step (x * y) (x' * y)
+  | beta_step_ap_right x y y' : beta_step y y' -> beta_step (x * y) (x * y')
+  | beta_step_i x : beta_step (I * x) x
+  | beta_step_k x y : beta_step (K * x * y) x
+  | beta_step_s x y z : beta_step (S * x * y * z) (x * z * (y * z)).
+Hint Constructors beta_step.
 
 Inductive test : code -> code -> Prop :=
   | test_refl x : test x x
@@ -35,6 +43,18 @@ Inductive test : code -> code -> Prop :=
 
 Definition conv (x : code) : Prop :=
   exists y z, probe x y /\ beta y z /\ test z TOP.
+
+Lemma beta_beta_step : forall x y, beta_step x y -> beta x y.
+Proof.
+  intros x y H; induction H; auto.
+Qed.
+
+Lemma beta_closed (p : code -> Prop) :
+  (forall x y, beta_step x y -> p x -> p y) ->
+  forall x y, beta x y -> p x -> p y.
+Proof.
+  intros Hs x y Hb; induction Hb; auto.
+Admitted.
 
 (* -------------------------------------------------------------------------- *)
 (* head function *)
@@ -71,7 +91,7 @@ Proof.
   congruence.
 Qed.
 
-Lemma not_conv_bot : ~conv BOT.
+Lemma not_conv_bot : ~ conv BOT.
 Proof.
   apply not_conv_head_bot; compute; auto.
 Qed.
@@ -114,7 +134,40 @@ Proof.
   inversion H; auto.
 Qed.
 
-Lemma not_conv_bot' : ~conv BOT.
+Lemma not_conv_bot' : ~ conv BOT.
 Proof.
   apply not_conv_heads_bot; heads.
 Qed.
+
+Definition Omega := (S * I * I) * (S * I * I).
+
+Definition Omega_beta (x : code) :=
+  x = (I * (S * I * I) * (I * (S * I * I))) \/
+  x = ((S * I * I) * (I * (S * I * I))) \/
+  x = (I * (S * I * I) * (S * I * I)) \/
+  x = ((S * I * I) * (S * I * I))
+.
+Hint Unfold Omega_beta.
+
+Definition Omega_heads (x : code) :=
+  heads (I * (S * I * I) * (I * (S * I * I))) x \/
+  heads ((S * I * I) * (I * (S * I * I))) x \/
+  heads (I * (S * I * I) * (S * I * I)) x \/
+  heads ((S * I * I) * (S * I * I)) x.
+
+Ltac beta_step :=
+  auto;
+  match goal with
+  | [H : beta_step ?x ?y |- _] => inversion_clear H; beta_step || idtac
+  end.
+
+Lemma beta_omega x y : beta x y -> Omega_beta x -> Omega_beta y.
+Proof.
+  apply beta_closed; intros.
+  destruct H0 as [o1|[o2|[o3|o4]]]; subst; auto; beta_step.
+  (* FIXME reduced to (I * (I * (S * I * I)) * (I * (I * (S * I * I)))) *)
+Admitted.
+
+Lemma not_conv_omega : ~ conv Omega.
+Proof.
+Admitted.
